theories/DeadCodeElimination/UCE.v
@@ -534,6 +534,10 @@ Proof.
   intros UC Ann LS.
   general induction LS; inv UC; simpl in *; eauto using true_live_sound.
   - econstructor; eauto using compile_live_incl with cset.
+    cases; eauto.
+    rewrite compile_live_incl in *; eauto. cases in H; eauto.
+    cases in H; eauto.
+    rewrite compile_live_incl in NOTCOND; eauto. cases in H; eauto.
     intros. eapply H. destruct H1; eauto.
     left. eapply compile_live_incl; eauto.
   - repeat cases.
